Some updates on paper and on lean development

lean/src/theory.lean
@@ -1,4 +1,7 @@
-import syntax semantics tactic.induction
+import syntax
+       semantics
+       tactic.induction
+       data.list.perm
 
 section theory
 
@@ -11,9 +14,13 @@ section theory
 
   inductive modal_theory (M : model) : list formula → Prop
   | nil_theory : modal_theory nil
-  | cons_theory : ∀ Γ φ, validate_model M φ → modal_theory Γ → modal_theory (cons φ Γ)
+  | cons_theory : ∀ Γ φ, validate_model M φ →
+                         modal_theory Γ →
+                         modal_theory (φ :: Γ)
 
-  def entails (M : model)(Γ : list formula)(φ : formula) : Prop
+  def entails (M : model)
+              (Γ : list formula)
+              (φ : formula) : Prop
     := modal_theory M Γ → validate_model M φ
 
   notation M `;;` Γ `⊢` φ := entails M Γ φ
@@ -21,7 +28,8 @@ section theory
   section structural_properties
 
     theorem exact_deduction
-      : ∀ (Γ : list formula)(φ : formula), φ ∈ Γ → ∀ (M : model), M ;; Γ ⊢ φ :=
+      : ∀ (Γ : list formula)(φ : formula),
+          φ ∈ Γ → ∀ (M : model), M ;; Γ ⊢ φ :=
     begin
       intros Γ,
       induction' Γ,
@@ -35,7 +43,8 @@ section theory
      end
 
      theorem refl_deduction 
-       : ∀ M Γ φ, modal_theory M (φ :: Γ) → (M ;; (φ :: Γ) ⊢ φ)
+       : ∀ M Γ φ, modal_theory M (φ :: Γ) →
+                  (M ;; (φ :: Γ) ⊢ φ)
      := by simp [exact_deduction]
 
 
@@ -55,6 +64,125 @@ section theory
          split ; try { constructor } ; assumption }
      end
 
+
+     theorem transitive_deduction_bu
+       : ∀ M Γ Δ φ₁ φ₂ φ₃,
+         (M ;; (φ₁ :: Γ) ⊢ φ₂) →
+         (M ;; (φ₂ :: Δ) ⊢ φ₃) →
+         (M ;; (φ₁ :: Γ ++ Δ) ⊢ φ₃) :=
+     begin
+       intros M Γ Δ φ₁ φ₂ φ₃ H1 H2 HM,
+       simp * at *,
+       have HMA : modal_theory M (φ₁ :: Γ) ∧ modal_theory M Δ,
+         from by { apply modal_theory_union, simp * at * },
+       cases HMA with HM1 HM2,
+       apply H2,
+       constructor ; try { assumption },
+       apply H1, try { assumption }
+     end
+
+     theorem exchange
+       : ∀ M Γ φ₁ φ₂ φ₃,
+         (M ;; (φ₁ :: φ₂ :: Γ) ⊢ φ₃) →
+         (M ;; (φ₂ :: φ₁ :: Γ) ⊢ φ₃) :=
+     begin
+       intros M Γ φ₁ φ₂ φ₃ H H1,
+       cases H1 with M Γ H2 H3,
+       cases H3 with M Γ H4 H5,
+       apply H,
+       repeat { constructor <|> assumption }
+     end
+
+     lemma modal_theory_permutation
+       : ∀ M Γ Δ, Γ ~ Δ → modal_theory M Γ → modal_theory M Δ :=
+       begin
+         intros M Γ Δ H1 H2,
+         induction' H1,
+         case list.perm.nil
+           { assumption },
+         case list.perm.cons
+           { cases H2,
+             constructor,
+             { assumption },
+             { apply ih, assumption }},
+         case list.perm.swap
+           { cases H2 with M Γ H21 H22,
+             cases H22 with M Γ H23 H24,
+             repeat { constructor <|> assumption }}, 
+         case list.perm.trans
+           { apply ih_H1_1,
+             apply ih_H1,
+             assumption}
+       end
+
+     theorem permutation_deduction
+       : ∀ M Γ Δ φ,
+       Γ ~ Δ →
+       (M ;; Γ ⊢ φ) →
+       (M ;; Δ ⊢ φ)
+     := begin
+          intros M Γ Δ φ H,
+          induction' H,
+          case list.perm.nil 
+             { intros H1 , assumption },
+          case list.perm.cons
+             { intros H1 HM1,
+               cases HM1 with M Δ HM11 HM12,
+               have HD1 : modal_theory M (x :: Γ),
+               from begin
+                      constructor,
+                      assumption,
+                      apply modal_theory_permutation ; try { assumption },
+                      apply list.perm.symm,
+                      assumption
+                    end,
+               apply H1, assumption},
+          case list.perm.swap
+            { intros H1 HM,
+              cases HM with M Δ HM1 HM2,
+              cases HM2 with M Δ HM3 HM4,
+              apply H1,
+              repeat { constructor <|> assumption }},
+          case list.perm.trans
+            { intros HM,
+              apply ih_H_1,
+              apply ih_H,
+              assumption }
+        end
+
+    theorem contraction
+      : ∀ M Γ φ₁ φ₂,
+        (M ;; (φ₁ :: φ₁ :: Γ) ⊢ φ₂) →
+        (M ;; (φ₁ :: Γ) ⊢ φ₂) :=
+    begin
+      intros M Γ φ₁ φ₂ H HM,
+      cases HM with M Γ HM1 HM2,
+      apply H,
+      repeat { constructor <|> assumption }
+    end
+
+    theorem monotonicity
+      : ∀ M Γ Δ φ,
+        (M ;; Γ ⊢ φ) →
+        (M ;; (Γ ++ Δ) ⊢ φ) :=
+    begin
+      intros M Γ Δ φ H HM,
+      apply H,
+      have HM1 : modal_theory M Γ ∧ modal_theory M Δ,
+        from by { apply modal_theory_union, assumption },
+      cases HM1, assumption
+    end
   end structural_properties
+
+  def entails_modal (Γ : list formula)(φ : formula) : Prop :=
+    ∀ M, modal_theory M Γ → validate_model M φ
+
+  def equivalence (φ₁ φ₂ : formula) : Prop :=
+    (entails_modal (φ₁ :: nil) φ₂) ∧
+    (entails_modal (φ₂ :: nil) φ₁)
+
+  notation φ₁ `.=.` φ₂ := equivalence φ₁ φ₂
+  notation Γ `⊩` φ := entails_modal Γ φ
   end list
 end theory
+
