lean/src/frame_completeness.lean
@@ -1,0 +1,21 @@
+import syntax
+       semantics
+       frame_properties
+
+
+section completeness
+  open modal_syntax
+  open model
+  open frame
+  open modal_syntax.formula
+
+  theorem reflexive_frame_completeness
+    : ∀ M φ, (M ⊧ ((.□ φ) .⟶. φ)) →
+             reflexivity_frame (F M) :=
+  begin
+    intros M φ H w,
+    simp [validate_model] at H,
+    simp [fun_validation] at H,
+    sorry
+  end
+end completeness
