lean/src/frame_properties.lean
@@ -1,0 +1,36 @@
+import syntax
+       semantics
+
+section properties
+
+  open modal_syntax
+  open model
+  open frame
+  open modal_syntax.formula
+
+  def reflexivity_frame (F : frame) : Prop :=
+    ∀ w, R F w w
+
+  def transitivity_frame (F : frame) : Prop :=
+    ∀ w₁ w₂ w₃, R F w₁ w₂ → R F w₂ w₃ → R F w₁ w₃
+
+  def simmetry_frame (F : frame) : Prop :=
+    ∀ w₁ w₂, R F w₁ w₂ → R F w₂ w₁
+
+  def euclidean_frame (F : frame) : Prop :=
+    ∀ w₁ w₂ w₃, R F w₁ w₂ → R F w₁ w₃ → R F w₂ w₃
+
+  def serial_frame (F : frame) : Prop :=
+    ∀ w, ∃ w', R F w w'
+
+  def functional_frame (F : frame) : Prop :=
+    ∀ w₁ w₂ w₃, R F w₁ w₂ →
+                R F w₁ w₃ →
+                w₂ = w₃
+
+  def dense_frame (F : frame) : Prop :=
+    ∀ w₁ w₂, ∃ w₃, R F w₁ w₂ → R F w₁ w₃ ∧ R F w₂ w₃
+
+  def convergent_frame (F : frame) : Prop :=
+    ∀ w x y, ∃ z, (R F w x ∧ R F w y) → (R F x z ∧ R F y z)
+end properties
