lean/src/frame_soundness.lean
@@ -1,0 +1,109 @@
+import syntax
+       semantics
+       frame_properties
+
+
+section soundness
+  open modal_syntax
+  open model
+  open frame
+  open modal_syntax.formula
+
+  theorem reflexive_frame_soundness
+    : ∀ M φ, reflexivity_frame (F M) →
+             (M ⊧ ((.□ φ) .⟶. φ)) :=
+  begin
+    intros M φ HR w,
+    rw reflexivity_frame at HR,
+    simp [fun_validation],
+    intros H,
+    apply H ; try {assumption},
+    apply HR
+  end
+
+  theorem transitive_frame_soundness
+    : ∀ M φ, transitivity_frame (F M) →
+             (M ⊧ ((.□ φ) .⟶. (.□ (.□ φ)))) :=
+  begin
+    intros M φ HT w,
+    rw transitivity_frame at HT,
+    simp [fun_validation],
+    intros H1 w₁ Hww₁ w₂ Hww₂,
+    apply H1,
+    { assumption }
+  end
+
+  theorem symmetry_frame_soundness
+    : ∀ M φ, simmetry_frame (F M) →
+             (M ⊧ (φ .⟶. (.□ (.◇ φ)))) :=
+  begin
+    intros M φ HS w,
+    rw simmetry_frame at HS,
+    simp [fun_validation],
+    intros H w' Hww',
+    split ; try {assumption},
+    constructor, {assumption}
+  end
+
+  theorem euclidean_frame_soundness
+    : ∀ M φ, euclidean_frame (F M) →
+             (M ⊧ (.◇ φ .⟶. (.□ (.◇ φ)))) :=
+  begin
+    intros M φ HE w,
+    rw euclidean_frame at HE,
+    simp [fun_validation],
+    intros w1 Hww1 H1 w2 Hww2,
+    split ; try { assumption },
+    constructor, { assumption }
+  end
+
+  theorem serial_frame_soundness
+    : ∀ M φ, serial_frame (F M) →
+             (M ⊧ ((.□ φ) .⟶. (.◇ φ))) :=
+  begin
+    intros M φ HS w,
+    rw serial_frame at HS,
+    simp [fun_validation],
+    intros H,
+    have H1 : ∃ w', M.F.R w w', from
+      by apply HS,
+    cases H1,
+    split,
+    { constructor, assumption },
+    { apply H, {assumption}}
+  end
+
+  theorem functional_frame_soundness
+    : ∀ M φ, functional_frame (F M) →
+             (M ⊧ ((.◇ φ) .⟶. (.□ φ))) :=
+  begin
+    intros M φ HF w,
+    simp [fun_validation],
+    intros w1 Hww1 H1 w2 Hww2,
+    assumption
+  end
+
+  theorem dense_frame_soundness
+    : ∀ M φ, dense_frame (F M) →
+          (M ⊧ ((.◇ (.□ φ)) .⟶. (.◇ φ))) :=
+  begin
+    intros M φ HD w,
+    simp [fun_validation],
+    intros w1 Hww1 H2,
+    split,
+    { constructor ; try { assumption }},
+    { apply H2 ; assumption }
+  end
+
+  theorem convergent_frame_soundness
+    : ∀ M φ, convergent_frame (F M) →
+     (M ⊧ ((.◇ (.□ φ)) .⟶. (.□ (.◇ φ)))) :=
+  begin
+    intros M φ HC w,
+    simp [fun_validation],
+    intros w1 Hww1 H1 w2 Hww2,
+    split,
+    {constructor ; try { assumption }},
+    {apply H1 ; try {assumption}}
+  end
+end soundness
